src/coq_formalism/example.v
@@ -5,844 +5,845 @@
  graphs to ensure our definitions 
  are correct *)
 
-Require Import Coq.Lists.List.
+ Require Import Coq.Lists.List.
 
-Require Import Order.attack_graph.
-Require Import Order.graph_strict_partial_order.
-Require Import Order.graph_normalization.
-Require Import Order.graph_equiv.
-Require Import Order.utilities.
-Require Import Order.graph_partial_order.
-Require Import Order.set_order.
-Require Import Order.compare. 
-
-
-(* ******************* 
-     sys & 
-   ker-vc-sys-seq 
-************************
-   Proving ker vc sys seq 
-   supports sys 
- * ****************** *)
-Module vc_sys_seq_supports_sys. 
-
-    Set Implicit Arguments.
-
-    Inductive measurement : Type :=
-    | ms : measurement
-    | ms4 : measurement.
-
-    Inductive adversary : Type :=
-    | sys : adversary
-    | ker : adversary
-    | vc : adversary
-    | a : adversary
-    | c : adversary.
-
-    Inductive states_sys : Type :=
-    | sys_sys : states_sys 
-    | sys_ker : states_sys
-    | sys_vc : states_sys
-    | sys_a : states_sys
-    | sys_c : states_sys
-    | sys_ms3 : states_sys
-    | sys_ms4 : states_sys.
-
-    Definition label_sys (st : states_sys) : measurement + adversary :=
-    match st with
-    | sys_sys => inr sys
-    | sys_ker => inr ker
-    | sys_vc => inr vc
-    | sys_a => inr a
-    | sys_c => inr c
-    | sys_ms3 => inl ms
-    | sys_ms4 => inl ms4
-    end.
-
-    (* 2 graphs for sys... m1a and m2a *)
-    Definition steps_m1a : list (states_sys * states_sys) := 
-        (sys_sys, sys_ms4) :: 
-        (sys_vc, sys_ms4) ::
-        nil.
-    
-    Definition m1a : attackgraph measurement adversary := 
-    {|
-        state := states_sys ;
-        steps := steps_m1a ;
-        label := label_sys
-    |}.
-
-    Definition steps_m2a : list (states_sys * states_sys) := 
-        (sys_sys, sys_ms4) :: 
-        (sys_ker, sys_ms4) ::
-        nil.
-    
-    Definition m2a : attackgraph measurement adversary := 
-    {|
-        state := states_sys ;
-        steps := steps_m2a ;
-        label := label_sys
-    |}.
-
-    Inductive states_vc_sys_seq : Type :=
-    | vc_sys_sys : states_vc_sys_seq 
-    | vc_sys_ker : states_vc_sys_seq
-    | vc_sys_vc : states_vc_sys_seq
-    | vc_sys_a : states_vc_sys_seq
-    | vc_sys_c : states_vc_sys_seq
-    | vc_sys_ms3 : states_vc_sys_seq
-    | vc_sys_ms4 : states_vc_sys_seq.
-
-    Definition label_vc_sys_seq (st : states_vc_sys_seq) : measurement + adversary :=
-    match st with
-    | vc_sys_sys => inr sys
-    | vc_sys_ker => inr ker
-    | vc_sys_vc => inr vc
-    | vc_sys_a => inr a
-    | vc_sys_c => inr c 
-    | vc_sys_ms3 => inl ms 
-    | vc_sys_ms4 => inl ms4
-    end.
-
-    (* 4 possible graphs *)
-
-    Definition steps_m1b : list (states_vc_sys_seq * states_vc_sys_seq) := 
-        (vc_sys_ms3, vc_sys_vc) :: 
-        (vc_sys_vc, vc_sys_ms4) ::
-        (vc_sys_sys, vc_sys_ms4) ::
-        nil.
-
-    Definition m1b : attackgraph measurement adversary := 
-    {|
-        state := states_vc_sys_seq ;
-        steps := steps_m1b ;
-        label := label_vc_sys_seq
-    |}.
-
-    Definition steps_m2b : list (states_vc_sys_seq * states_vc_sys_seq) := 
-        (vc_sys_ms3, vc_sys_ms4) :: 
-        (vc_sys_vc, vc_sys_ms4) ::
-        (vc_sys_sys, vc_sys_ms4) ::
-        nil.
-
-    Definition m2b : attackgraph measurement adversary := 
-    {|
-        state := states_vc_sys_seq ;
-        steps := steps_m2b ;
-        label := label_vc_sys_seq
-    |}.
-
-    Definition steps_m3b : list (states_vc_sys_seq * states_vc_sys_seq) := 
-        (vc_sys_vc, vc_sys_ms3) ::
-        (vc_sys_a, vc_sys_ms3) ::
-        (vc_sys_ms3, vc_sys_ms4) :: 
-        (vc_sys_sys, vc_sys_ms4) ::
-        nil.
-
-    Definition m3b : attackgraph measurement adversary := 
-    {|
-        state := states_vc_sys_seq ;
-        steps := steps_m3b ;
-        label := label_vc_sys_seq
-    |}.
-
-    Definition steps_m4b : list (states_vc_sys_seq * states_vc_sys_seq) := 
-        (vc_sys_vc, vc_sys_ms3) ::
-        (vc_sys_c, vc_sys_ms3) ::
-        (vc_sys_ms3, vc_sys_ms4) :: 
-        (vc_sys_sys, vc_sys_ms4) ::
-        nil.
-
-    Definition m4b : attackgraph measurement adversary := 
-    {|
-        state := states_vc_sys_seq ;
-        steps := steps_m4b ;
-        label := label_vc_sys_seq
-    |}.
-
-    (* Prove m2b, m3b and m4b reduce *)
-
-    Definition steps_m2b' : list (states_vc_sys_seq * states_vc_sys_seq) := 
-        (vc_sys_vc, vc_sys_ms4) ::
-        (vc_sys_sys, vc_sys_ms4) ::
-        nil.
-
-    Definition m2b' : attackgraph measurement adversary := 
-    {|
-        state := states_vc_sys_seq ;
-        steps := steps_m2b' ;
-        label := label_vc_sys_seq
-    |}.
-
-    Definition steps_m3b' : list (states_vc_sys_seq * states_vc_sys_seq) := 
-        (vc_sys_vc, vc_sys_ms4) ::
-        (vc_sys_a, vc_sys_ms4) ::
-        (vc_sys_sys, vc_sys_ms4) ::
-        nil.
-
-    Definition m3b' : attackgraph measurement adversary := 
-    {|
-        state := states_vc_sys_seq ;
-        steps := steps_m3b' ;
-        label := label_vc_sys_seq
-    |}.
-
-    Definition steps_m4b' : list (states_vc_sys_seq * states_vc_sys_seq) := 
-        (vc_sys_vc, vc_sys_ms4) ::
-        (vc_sys_c, vc_sys_ms4) ::
-        (vc_sys_sys, vc_sys_ms4) ::
-        nil.
-
-    Definition m4b' : attackgraph measurement adversary := 
-    {|
-        state := states_vc_sys_seq ;
-        steps := steps_m4b' ;
-        label := label_vc_sys_seq
-    |}.
-
-    Lemma eqDec_measurement : forall (x y : measurement), {x = y} + {x <> y}.
-    Proof. destruct x, y; try (left; reflexivity); try (right; intros contra; inversion contra). Qed.
-    Lemma eqDec_adversary : forall (x y : adversary), {x = y} + {x <> y}.
-    Proof. destruct x, y; try (left; reflexivity); try (right; intros contra; inversion contra). Qed.
-    Lemma eqDec_state2: forall (x y : m2b.(state _ _)), {x = y} + {x <> y}.
-    Proof. destruct x, y; try (left; reflexivity); try (right; intros contra; inversion contra). Qed.
-    Lemma eqDec_state3: forall (x y : m3b.(state _ _)), {x = y} + {x <> y}.
-    Proof. destruct x, y; try (left; reflexivity); try (right; intros contra; inversion contra). Qed.
-    Lemma eqDec_state4: forall (x y : m4b.(state _ _)), {x = y} + {x <> y}.
-    Proof. destruct x, y; try (left; reflexivity); try (right; intros contra; inversion contra). Qed.
-
-    Ltac eqDec_step_left step1 step2 eqDec_state :=
-    destruct (eqDec_step eqDec_state step1 step2) as [H|H]; [clear H | contradiction].
-    Ltac eqDec_step_right step1 step2 eqDec_state :=
-    destruct (eqDec_step eqDec_state step1 step2) as [H|H]; [inversion H | clear H].
-    Ltac eqDec_state_left st1 st2 eqDec_state :=
-    destruct (eqDec_state st1 st2) as [H|H]; [clear H | contradiction].
-    Ltac eqDec_state_right st1 st2 eqDec_state :=
-    destruct (eqDec_state st1 st2) as [H|H]; [inversion H | clear H].
-
-    Lemma example_m2b_reduce1 : 
-    reduce1 eqDec_state2 steps_m2b =
-    steps_m2b'.
-    Proof.
-     unfold reduce1. simpl. 
-     eqDec_step_left (vc_sys_ms3, vc_sys_ms4) (vc_sys_ms3, vc_sys_ms4) eqDec_state2.
-     eqDec_step_right (vc_sys_ms3, vc_sys_ms4) (vc_sys_vc, vc_sys_ms4) eqDec_state2.
-     eqDec_step_right (vc_sys_ms3, vc_sys_ms4) (vc_sys_sys, vc_sys_ms4) eqDec_state2.
-     simpl.
-     eqDec_state_right vc_sys_vc vc_sys_ms3 eqDec_state2.
-     eqDec_state_right vc_sys_ms4 vc_sys_ms3 eqDec_state2.
-     eqDec_state_right vc_sys_sys vc_sys_ms3 eqDec_state2.
-     unfold steps_m2b'. reflexivity.
-    Qed. 
-
-    Lemma m2b_reduced : reducer eqDec_state2 steps_m2b steps_m2b'.
-    Proof. 
-        apply reduce_more.
-        + rewrite example_m2b_reduce1. unfold not. intros. inversion H. 
-        + rewrite example_m2b_reduce1. apply reduce_done. eauto.
-    Qed. 
-
-    Lemma example_m3b_reduce1 : 
-    reduce1 eqDec_state3 steps_m3b =
-    steps_m3b'.
-    Proof.
-     unfold reduce1. simpl. 
-     eqDec_step_right (vc_sys_ms3, vc_sys_ms4) (vc_sys_vc, vc_sys_ms3) eqDec_state3.
-     eqDec_step_right (vc_sys_ms3, vc_sys_ms4) (vc_sys_a, vc_sys_ms3) eqDec_state3.
-     eqDec_step_left (vc_sys_ms3, vc_sys_ms4) (vc_sys_ms3, vc_sys_ms4) eqDec_state3.
-     eqDec_step_right (vc_sys_ms3, vc_sys_ms4) (vc_sys_sys, vc_sys_ms4) eqDec_state3.
-     simpl.
-     eqDec_state_right vc_sys_vc vc_sys_ms3 eqDec_state3.
-     eqDec_state_right vc_sys_a vc_sys_ms3 eqDec_state3.
-     eqDec_state_left vc_sys_ms3 vc_sys_ms3 eqDec_state3.
-     eqDec_state_right vc_sys_sys vc_sys_ms3 eqDec_state3.
-     eqDec_state_right vc_sys_ms4 vc_sys_ms3 eqDec_state3.
-     unfold steps_m3b'. reflexivity.
-    Qed. 
-
-    Lemma m3b_reduced : reducer eqDec_state3 steps_m3b steps_m3b'.
-    Proof. 
-        apply reduce_more.
-        + rewrite example_m3b_reduce1. unfold not. intros. inversion H. 
-        + rewrite example_m3b_reduce1. apply reduce_done. eauto.
-    Qed. 
-
-    Lemma example_m4b_reduce1 : 
-    reduce1 eqDec_state4 steps_m4b =
-    steps_m4b'.
-    Proof.
-     unfold reduce1. simpl. 
-     eqDec_step_right (vc_sys_ms3, vc_sys_ms4) (vc_sys_vc, vc_sys_ms3) eqDec_state4.
-     eqDec_step_right (vc_sys_ms3, vc_sys_ms4) (vc_sys_c, vc_sys_ms3) eqDec_state4.
-     eqDec_step_left (vc_sys_ms3, vc_sys_ms4) (vc_sys_ms3, vc_sys_ms4) eqDec_state4.
-     eqDec_step_right (vc_sys_ms3, vc_sys_ms4) (vc_sys_sys, vc_sys_ms4) eqDec_state4.
-     simpl.
-     eqDec_state_right vc_sys_vc vc_sys_ms3 eqDec_state4.
-     eqDec_state_right vc_sys_c vc_sys_ms3 eqDec_state4.
-     eqDec_state_left vc_sys_ms3 vc_sys_ms3 eqDec_state4.
-     eqDec_state_right vc_sys_sys vc_sys_ms3 eqDec_state4.
-     eqDec_state_right vc_sys_ms4 vc_sys_ms3 eqDec_state4.
-     unfold steps_m4b'. reflexivity.
-    Qed. 
-
-    Lemma m4b_reduced : reducer eqDec_state4 steps_m4b steps_m4b'.
-    Proof. 
-        apply reduce_more.
-        + rewrite example_m4b_reduce1. unfold not. intros. inversion H. 
-        + rewrite example_m4b_reduce1. apply reduce_done. eauto.
-    Qed.
-
-    (* define isomorphism function *)
-    Definition f (x : states_sys) : states_vc_sys_seq :=
-        match x with 
-        | sys_sys => vc_sys_sys 
-        | sys_vc => vc_sys_vc
-        | sys_ker => vc_sys_ker
-        | sys_a => vc_sys_a
-        | sys_c => vc_sys_c
-        | sys_ms3 => vc_sys_ms3
-        | sys_ms4 => vc_sys_ms4
-    end.
-
-    Definition g (x : states_vc_sys_seq) : option (states_sys) :=
-        match x with 
-        | vc_sys_sys => Some sys_sys 
-        | vc_sys_vc => Some sys_vc
-        | vc_sys_ker => Some sys_ker
-        | vc_sys_ms4 => Some sys_ms4
-        | _ => None
-    end.
-
-    Definition g' (x : states_vc_sys_seq) : (states_sys) :=
-        match x with 
-        | vc_sys_sys =>  sys_sys 
-        | vc_sys_vc =>  sys_vc
-        | vc_sys_ker =>  sys_ker
-        | vc_sys_ms4 =>  sys_ms4
-        | _ => sys_ms4
-    end.
-    
-    Definition sys_all : list (attackgraph measurement adversary) :=  m1a :: m2a :: nil .
-
-    Definition vc_sys_seq_all := m1b :: m2b' :: m3b' :: m4b' :: nil.
-
-    Ltac cor_in_head := simpl; apply ex_head; auto.
-    Ltac cor_in_tail := simpl; apply ex_tail; auto.
-
-    Lemma m1a_supports_m1b : supports ( m1a :: nil ) (m1b :: nil).
-    Proof.
-        unfold supports. intros. simpl in H0. intuition. 
-        exists m1a. simpl in *. split.
-        + left. reflexivity.
-        + right. subst. unfold strict_partial_order. intuition.
-        ++ econstructor.
-        +++ simpl. unfold steps_m1b. apply ex_tail. apply ex_tail. apply ex_head. simpl. intuition.
-        +++  econstructor. simpl. unfold steps_m1b. apply ex_tail. apply ex_head. simpl. eauto. econstructor.
-        ++ econstructor.
-        +++ simpl. unfold steps_m1b. unfold find_time. simpl. eauto.
-        +++ econstructor. simpl. unfold steps_m1b. unfold find_time. simpl. eauto.
-            econstructor.
-        ++ right. unfold time_proper_subset. split.
-        +++ econstructor.
-        ++++ simpl. unfold steps_m1b. unfold find_time. simpl. eauto.
-        ++++ econstructor. simpl. unfold steps_m1b. unfold find_time. simpl. eauto.
-            econstructor.
-        +++ unfold not. intros. invc H. subst. simpl in *. invc H2. subst.
-            simpl in *. destruct H0. inversion H0. subst. invc H0. subst. 
-            destruct H1. simpl in *. invc H. subst. invc H1.
-    Qed.
-
-    Ltac inversion_any :=
-      match goal with
-      | [H : _ |- _ ] => inversion H
-      end.
-
-    Lemma vc_sys_seq_supports_sys : supports sys_all vc_sys_seq_all.
-    Proof.
-      unfold supports. intros. simpl in H0. intuition.
-      + subst. exists m1a. unfold sys_all; intuition. right.
-        unfold strict_partial_order. intuition.
-      ++ econstructor. 
-      +++ simpl. unfold steps_m1b. apply ex_tail. apply ex_tail. apply ex_head. simpl. intuition.
-      +++ econstructor. simpl. unfold steps_m1b. apply ex_tail. apply ex_head. simpl. eauto. econstructor.
-      ++ econstructor.
-      +++ simpl. unfold steps_m1b. unfold find_time. simpl. eauto.
-      +++ econstructor. simpl. unfold steps_m1b. unfold find_time. simpl. eauto.
-          econstructor.
-      ++ right. unfold time_proper_subset. split.
-      +++ econstructor.
-      ++++ simpl. unfold steps_m1b. unfold find_time. simpl. eauto.
-      ++++ econstructor. simpl. unfold steps_m1b. unfold find_time. simpl. eauto.
-          econstructor.
-      +++ unfold not. intros. invc H. subst. simpl in *. invc H2. subst.
-          simpl in *. destruct H0. inversion H0. subst. invc H0. subst. 
-          destruct H1. simpl in *. invc H. subst. invc H1.
-      + subst. exists m1a. unfold sys_all. intuition. left.
-        unfold isomorphism. exists f. unfold f. repeat split; intros.
-      ++ destruct st1, st2; try (simpl in *; intuition; inversion_any).
-      ++ destruct st1, st2; try (simpl in *; intuition; inversion_any).
-      ++ destruct st; auto.
-      ++ destruct st1, st2; try reflexivity; inversion_any.
-      ++ destruct st'.
-      +++ exists sys_sys; reflexivity.
-      +++ exists sys_ker; reflexivity.
-      +++ exists sys_vc; reflexivity.
-      +++ exists sys_a; reflexivity.
-      +++ exists sys_c; reflexivity.
-      +++ exists sys_ms3; reflexivity.
-      +++ exists sys_ms4; reflexivity.
-      + exists m1a. unfold sys_all. intuition. right. subst.
-        unfold strict_partial_order. intuition. 
-      ++  econstructor. 
-      +++ simpl. unfold steps_m3b'. apply ex_tail. apply ex_tail. apply ex_head. simpl. intuition.
-      +++ econstructor. simpl. unfold steps_m3b'. apply ex_head. simpl. eauto. econstructor.
-      ++ econstructor.
-      +++ simpl. unfold steps_m3b'. unfold find_time. simpl. eauto.
-      +++ econstructor. simpl. unfold steps_m3b'. unfold find_time. simpl. eauto.
-          econstructor.
-      ++ left. unfold cor_proper_subset. intuition.
-      +++ econstructor.  
-      ++++ simpl. unfold steps_m3b'. apply ex_tail. apply ex_tail. apply ex_head. simpl. intuition.
-      ++++ econstructor. simpl. unfold steps_m3b'. apply ex_head. simpl. eauto. econstructor.
-      +++ invc H. subst. invc H4. subst. invc H1. subst. invc H0.
-          subst. invc H0. subst. invc H1. invc H1.
-      +  exists m1a. unfold sys_all. intuition. right. subst.
-      unfold strict_partial_order. intuition. 
-    ++  econstructor. 
-    +++ simpl. unfold steps_m3b'. apply ex_tail. apply ex_tail. apply ex_head. simpl. intuition.
-    +++ econstructor. simpl. unfold steps_m3b'. apply ex_head. simpl. eauto. econstructor.
-    ++ econstructor.
-    +++ simpl. unfold steps_m3b'. unfold find_time. simpl. eauto.
-    +++ econstructor. simpl. unfold steps_m3b'. unfold find_time. simpl. eauto.
-        econstructor.
-    ++ left. unfold cor_proper_subset. intuition.
-    +++ econstructor.  
-    ++++ simpl. unfold steps_m3b'. apply ex_tail. apply ex_tail. apply ex_head. simpl. intuition.
-    ++++ econstructor. simpl. unfold steps_m3b'. apply ex_head. simpl. eauto. econstructor.
-    +++ invc H. subst. invc H4. subst. invc H1. subst. invc H0.
-        subst. invc H0. subst. invc H1. invc H1.
- Qed.
-
- (* TO DO... random example. Not part of dissertation. *)
- Theorem vc_sys_seq_set_reduced : reduce_set vc_sys_seq_all vc_sys_seq_all (m2b' :: nil).
- Proof.
-    unfold vc_sys_seq_all. apply set_remove. 
-    + exists m2b'. split; auto with *.  admit.
-    + apply set_keep.
-    ++ intros. simp_int.
-    +++ subst. unfold strict_partial_order in H0. invc H0. admit.
-    +++ subst.  admit.
-    +++ admit. 
-    +++ admit.
-    ++  apply set_remove. 
-    +++ exists m2b'.  admit.
-    +++ apply set_remove. 
-    ++++ admit.
-    ++++ apply set_nil.     
-Admitted.
+ Require Import Order.attack_graph.
+ Require Import Order.graph_strict_partial_order.
+ Require Import Order.graph_normalization.
+ Require Import Order.graph_equiv.
+ Require Import Order.utilities.
+ Require Import Order.graph_partial_order.
+ Require Import Order.set_order.
+ Require Import Order.compare. 
  
-
-End vc_sys_seq_supports_sys. 
-
-
-(* *********** *)
-(* Example m2c *)
-(* *********** *)
-(* *********** *)
-
-Module m3b.
-
-    Set Implicit Arguments.
-    
-    Inductive measurement : Type :=
-    | ms : measurement
-    | ms4 : measurement.
-    
-    Inductive adversary : Type :=
-    | sys : adversary
-    | ker : adversary.
-    
-    Inductive state_m3b : Type :=
-    | s : state_m3b 
-    | k : state_m3b
-    | m : state_m3b
-    | m4 : state_m3b.
-    
-    Definition label_m3b (st : state_m3b) : measurement + adversary :=
-    match st with
-    | s => inr sys
-    | k => inr ker
-    | m => inl ms
-    | m4 => inl ms4
-    end.
-    
-    Definition steps_m3b : list (state_m3b * state_m3b) := 
-        (k, m) :: 
-        (m, m4) ::
-        (s, m4) ::
-        nil.
-    
-    Definition m3b : attackgraph measurement adversary := 
-    {|
-        state := state_m3b ;
-        steps := steps_m3b ;
-        label := label_m3b
-    |}.
-    
-    Lemma eqDec_measurement : forall (x y : measurement), {x = y} + {x <> y}.
-    Proof. destruct x, y; try (left; reflexivity); try (right; intros contra; inversion contra). Qed.
-    Lemma eqDec_adversary : forall (x y : adversary), {x = y} + {x <> y}.
-    Proof. destruct x, y; try (left; reflexivity); try (right; intros contra; inversion contra). Qed.
-    Lemma eqDec_state: forall (x y : m3b.(state _ _)), {x = y} + {x <> y}.
-    Proof. destruct x, y; try (left; reflexivity); try (right; intros contra; inversion contra). Qed.
-
-    Ltac eqDec_step_left step1 step2 :=
-    destruct (eqDec_step eqDec_state step1 step2) as [H|H]; [clear H | contradiction].
-    Ltac eqDec_step_right step1 step2 :=
-    destruct (eqDec_step eqDec_state step1 step2) as [H|H]; [inversion H | clear H].
-    Ltac eqDec_state_left st1 st2 :=
-    destruct (eqDec_state st1 st2) as [H|H]; [clear H | contradiction].
-    Ltac eqDec_state_right st1 st2 :=
-    destruct (eqDec_state st1 st2) as [H|H]; [inversion H | clear H].
-
-    Print reduce1.
-
-    Lemma example_m3b : 
-    (reduce1 eqDec_state m3b.(steps _ _)) =
-    ((k, m4) :: (s, m4) :: nil).
-    Proof.
-        unfold reduce1.
-        simpl. 
-        eqDec_step_right (m, m4) (k, m).
-        eqDec_step_left (m, m4) (m, m4).
-        eqDec_step_right (m, m4) (s, m4).
-        simpl.
-        eqDec_state_right k m.
-        eqDec_state_left m m.
-        eqDec_state_right s m.
-        eqDec_state_right m4 m.
-        eauto.
-    Qed.
-
-    Definition m3b_steps := m3b.(steps _ _).
-    Definition m3b_reduced := ((k, m4) :: (s, m4) :: nil).
-
-    Check reducer eqDec_state m3b_steps m3b_reduced. 
-
-    Lemma example_m3b_reducer : 
-        reducer eqDec_state m3b_steps m3b_reduced.
-    Proof.
-        econstructor.
-        + unfold m3b_steps. rewrite example_m3b. simpl. intros contra. inversion contra.
-        + unfold m3b_steps. rewrite example_m3b.
-          apply reduce_done. unfold reduce1. simpl. eauto.
-    Qed.
-    
-
-End m3b.
-
-
-(* *********** *)
-(* Example m2c *)
-(* *********** *)
-(* *********** *)
-Module m2c.
-
-Inductive measurement : Type :=
-| ms : measurement
-| ms4 : measurement.
-
-Inductive adversary : Type :=
-| sys : adversary
-| ker : adversary.
-
-Inductive state_m2c : Type :=
-| s : state_m2c
-| k : state_m2c
-| m : state_m2c
-| m' : state_m2c
-| m4 : state_m2c.
-
-Definition label_m2c (st : state_m2c) : measurement + adversary :=
-match st with
-| s => inr sys
-| k => inr ker
-| m => inl ms
-| m' => inl ms
-| m4 => inl ms4
-end.
-
-Definition steps_m2c : list (state_m2c * state_m2c) :=  
-    (m, m') ::
-    (m', k) ::
-    (s, m4) :: 
-    (k, m4) :: 
-    nil.
-
-Definition steps_m2b : list (state_m2c * state_m2c) :=  
-    (m', k) ::
-    (s, m4) :: 
-    (k, m4) :: 
-    nil.
-
-Definition steps_m2a : list (state_m2c * state_m2c) :=  
-    (s, m4) :: 
-    (k, m4) :: 
-    nil.
-
-
-Definition m2c : attackgraph measurement adversary := 
-{|
-    state := state_m2c ;
-    steps := steps_m2c ;
-    label := label_m2c
-|}.
-
-Definition m2b : attackgraph measurement adversary := 
-{|
-    state := state_m2c ;
-    steps := steps_m2b ;
-    label := label_m2c
-|}.
-
-Definition m2a : attackgraph measurement adversary := 
-{|
-    state := state_m2c ;
-    steps := steps_m2a ;
-    label := label_m2c
-|}.
-
-Definition m2a_nil : attackgraph measurement adversary := 
-{|
-    state := state_m2c ;
-    steps := nil ;
-    label := label_m2c
-|}.
-
-
-Lemma eqDec_measurement : forall (x y : measurement), {x = y} + {x <> y}.
-Proof. destruct x, y; try (left; reflexivity); try (right; intros contra; inversion contra). Qed.
-Lemma eqDec_adversary : forall (x y : adversary), {x = y} + {x <> y}.
-Proof. destruct x, y; try (left; reflexivity); try (right; intros contra; inversion contra). Qed.
-Lemma eqDec_state : forall (x y : m2c.(state _ _)), {x = y} + {x <> y}.
-Proof. destruct x, y; try (left; reflexivity); try (right; intros contra; inversion contra). Qed.
-
-Ltac eqDec_step_left step1 step2 :=
-    destruct (eqDec_step eqDec_state step1 step2) as [H|H]; [clear H | contradiction].
-Ltac eqDec_step_right step1 step2 :=
-    destruct (eqDec_step eqDec_state step1 step2) as [H|H]; [inversion H | clear H].
-Ltac eqDec_state_left st1 st2 :=
-    destruct (eqDec_state st1 st2) as [H|H]; [clear H | contradiction].
-Ltac eqDec_state_right st1 st2 :=
-    destruct (eqDec_state st1 st2) as [H|H]; [inversion H | clear H].
-
-Lemma example_m2c : 
-    (reduce1 eqDec_state m2c.(steps _ _)) =
-    ((m', k) :: (s, m4) :: (k, m4) :: nil).
-Proof.
-    unfold reduce1.
-    simpl. 
-    eqDec_step_left (m, m') (m, m').
-    eqDec_step_right (m, m') (m', k).
-    eqDec_step_right (m, m') (s, m4).
-    eqDec_step_right (m, m') (k, m4).
-    simpl.
-    eqDec_state_right m' m.
-    eqDec_state_right k m.
-    eqDec_state_right s m.
-    eqDec_state_right m4 m.
-    reflexivity.
-Qed.
-
-Print time_subset. 
-Lemma time_subset_m2a_m2c : time_subset m2a.(steps _ _) m2c.(steps _ _).
-Proof.
-    simpl. auto.
-Qed.
-
-(* TODO: this proof?? *)
-Lemma not_time_subset_m2c_m2a : ~ time_subset m2c.(steps _ _) m2a.(steps _ _).
-Proof.
-    unfold not; intros.
-    inversion H. inversion H0.
-    inversion H2. clear H2.
-Abort.
-
-(* TODO: this proof too? *)
-Lemma subset_nil : ~ cor_subset m2a.(steps _ _) m2a_nil.(steps _ _).
-Proof.
-Abort.
-
-(* TODO *)
-Lemma subset_nil_with_meas : ~ cor_subset m2c.(steps _ _) m2a_nil.(steps _ _).
-Proof.
-Abort.
-
-End m2c.
-
-(* *********** *)
-(* Example m5c *)
-(* *********** *)
-(* *********** *)
-Module m5c.
-
-Inductive measurement : Type :=
-| ms : measurement
-| ms4 : measurement.
-
-Inductive adversary : Type :=
-| sys : adversary
-| vc : adversary
-| cc : adversary.
-
-Inductive state_m5c : Type :=
-| s : state_m5c
-| v : state_m5c
-| c : state_m5c
-| m : state_m5c
-| m' : state_m5c
-| m4 : state_m5c.
-
-Definition label_m5c (st : state_m5c) : measurement + adversary :=
-match st with
-| s => inr sys
-| v => inr vc
-| c => inr cc
-| m => inl ms
-| m' => inl ms
-| m4 => inl ms4
-end.
-
-Definition steps_m5c : list (state_m5c * state_m5c) := 
-    (c, m') ::
-    (m, m') ::
-    (v, m') ::
-    (m', m4) ::
-    (s, m4) ::
-    nil.
-
-Definition m5c : attackgraph measurement adversary := 
-{|
-    state := state_m5c ;
-    steps := steps_m5c ;
-    label := label_m5c
-|}.
-
-(* remove c to m' to have a proper subset *)
-Definition steps_m5c' : list (state_m5c * state_m5c) := 
-    (m, m') ::
-    (v, m') ::
-    (m', m4) ::
-    (s, m4) ::
-    nil.
-
-(* new graph that would be proper subset *)
-Definition m5c' : attackgraph measurement adversary := 
-{|
-    state := state_m5c ;
-    steps := steps_m5c' ;
-    label := label_m5c
-|}.
-
-Lemma eqDec_measurement : forall (x y : measurement), {x = y} + {x <> y}.
-Proof. destruct x, y; try (left; reflexivity); try (right; intros contra; inversion contra). Qed.
-Lemma eqDec_adversary : forall (x y : adversary), {x = y} + {x <> y}.
-Proof. destruct x, y; try (left; reflexivity); try (right; intros contra; inversion contra). Qed.
-Lemma eqDec_state : forall (x y : m5c.(state _ _)), {x = y} + {x <> y}.
-Proof. destruct x, y; try (left; reflexivity); try (right; intros contra; inversion contra). Qed.
-
-
-Ltac eqDec_step_left step1 step2 :=
-    destruct (eqDec_step eqDec_state step1 step2) as [H|H]; [clear H | contradiction].
-Ltac eqDec_step_right step1 step2 :=
-    destruct (eqDec_step eqDec_state step1 step2) as [H|H]; [inversion H | clear H].
-Ltac eqDec_state_left st1 st2 :=
-    destruct (eqDec_state st1 st2) as [H|H]; [clear H | contradiction].
-Ltac eqDec_state_right st1 st2 :=
-    destruct (eqDec_state st1 st2) as [H|H]; [inversion H | clear H].
-    
-Definition m5c_steps := m5c.(steps _ _).
-Definition m5c'_steps := m5c'.(steps _ _).
-Definition m5c_reduced := ((c, m4) :: (v, m4) :: (s, m4) :: nil).
-
-(* must call reduce1 twice here *)
-Lemma example_m5c' : 
-    (reduce1 eqDec_state (reduce1 eqDec_state m5c.(steps _ _))) =
-    ((c, m4) :: (v, m4) :: (s, m4) :: nil).
-Proof.
-    unfold reduce1.
-    simpl.
-    eqDec_step_right (m, m') (c, m').
-    eqDec_step_left (m, m') (m, m').
-    eqDec_step_right (m, m') (v, m').
-    eqDec_step_right (m, m') (m', m4).
-    eqDec_step_right (m, m') (s, m4).
-    simpl.
-    eqDec_state_right c m.
-    eqDec_state_right v m.
-    eqDec_state_right m' m.
-    eqDec_state_right m4 m.
-    eqDec_state_right s m.
-    simpl.
-    eqDec_step_right (m', m4) (c, m').
-    eqDec_step_right (m', m4) (v, m').
-    eqDec_step_left (m', m4) (m', m4).
-    eqDec_step_right (m', m4) (s, m4).
-    simpl.
-    eqDec_state_right c m'.
-    eqDec_state_left m' m'.
-    eqDec_state_right v m'.
-    eqDec_state_right s m'.
-    eqDec_state_right m4 m'.
-    reflexivity.
-Qed.
-
-Lemma example_m5c_reducer : 
-reducer eqDec_state m5c_steps m5c_reduced.
-Proof.
-    econstructor.
-    + unfold m5c_steps. simpl. unfold reduce1. simpl. 
-      eqDec_step_right (m, m') (c, m').
-      eqDec_step_left (m, m') (m, m').
-      eqDec_step_right (m, m') (v, m').
-      eqDec_step_right (m, m') (m', m4).
-      eqDec_step_right (m, m') (s, m4).
+ 
+ (* ******************* 
+      sys & 
+    ker-vc-sys-seq 
+ ************************
+    Proving ker vc sys seq 
+    supports sys 
+  * ****************** *)
+ Module vc_sys_seq_supports_sys. 
+ 
+     Set Implicit Arguments.
+ 
+     Inductive measurement : Type :=
+     | ms : measurement
+     | ms4 : measurement.
+ 
+     Inductive adversary : Type :=
+     | sys : adversary
+     | ker : adversary
+     | vc : adversary
+     | a : adversary
+     | c : adversary.
+ 
+     Inductive states_sys : Type :=
+     | sys_sys : states_sys 
+     | sys_ker : states_sys
+     | sys_vc : states_sys
+     | sys_a : states_sys
+     | sys_c : states_sys
+     | sys_ms3 : states_sys
+     | sys_ms4 : states_sys.
+ 
+     Definition label_sys (st : states_sys) : measurement + adversary :=
+     match st with
+     | sys_sys => inr sys
+     | sys_ker => inr ker
+     | sys_vc => inr vc
+     | sys_a => inr a
+     | sys_c => inr c
+     | sys_ms3 => inl ms
+     | sys_ms4 => inl ms4
+     end.
+ 
+     (* 2 graphs for sys... m1a and m2a *)
+     Definition steps_m1a : list (states_sys * states_sys) := 
+         (sys_sys, sys_ms4) :: 
+         (sys_vc, sys_ms4) ::
+         nil.
+     
+     Definition m1a : attackgraph measurement adversary := 
+     {|
+         event := states_sys ;
+         edges := steps_m1a ;
+         label := label_sys
+     |}.
+ 
+     Definition steps_m2a : list (states_sys * states_sys) := 
+         (sys_sys, sys_ms4) :: 
+         (sys_ker, sys_ms4) ::
+         nil.
+     
+     Definition m2a : attackgraph measurement adversary := 
+     {|
+         event := states_sys ;
+         edges := steps_m2a ;
+         label := label_sys
+     |}.
+ 
+     Inductive states_vc_sys_seq : Type :=
+     | vc_sys_sys : states_vc_sys_seq 
+     | vc_sys_ker : states_vc_sys_seq
+     | vc_sys_vc : states_vc_sys_seq
+     | vc_sys_a : states_vc_sys_seq
+     | vc_sys_c : states_vc_sys_seq
+     | vc_sys_ms3 : states_vc_sys_seq
+     | vc_sys_ms4 : states_vc_sys_seq.
+ 
+     Definition label_vc_sys_seq (st : states_vc_sys_seq) : measurement + adversary :=
+     match st with
+     | vc_sys_sys => inr sys
+     | vc_sys_ker => inr ker
+     | vc_sys_vc => inr vc
+     | vc_sys_a => inr a
+     | vc_sys_c => inr c 
+     | vc_sys_ms3 => inl ms 
+     | vc_sys_ms4 => inl ms4
+     end.
+ 
+     (* 4 possible graphs *)
+ 
+     Definition steps_m1b : list (states_vc_sys_seq * states_vc_sys_seq) := 
+         (vc_sys_ms3, vc_sys_vc) :: 
+         (vc_sys_vc, vc_sys_ms4) ::
+         (vc_sys_sys, vc_sys_ms4) ::
+         nil.
+ 
+     Definition m1b : attackgraph measurement adversary := 
+     {|
+         event := states_vc_sys_seq ;
+         edges := steps_m1b ;
+         label := label_vc_sys_seq
+     |}.
+ 
+     Definition steps_m2b : list (states_vc_sys_seq * states_vc_sys_seq) := 
+         (vc_sys_ms3, vc_sys_ms4) :: 
+         (vc_sys_vc, vc_sys_ms4) ::
+         (vc_sys_sys, vc_sys_ms4) ::
+         nil.
+ 
+     Definition m2b : attackgraph measurement adversary := 
+     {|
+         event := states_vc_sys_seq ;
+         edges := steps_m2b ;
+         label := label_vc_sys_seq
+     |}.
+ 
+     Definition steps_m3b : list (states_vc_sys_seq * states_vc_sys_seq) := 
+         (vc_sys_vc, vc_sys_ms3) ::
+         (vc_sys_a, vc_sys_ms3) ::
+         (vc_sys_ms3, vc_sys_ms4) :: 
+         (vc_sys_sys, vc_sys_ms4) ::
+         nil.
+ 
+     Definition m3b : attackgraph measurement adversary := 
+     {|
+         event := states_vc_sys_seq ;
+         edges := steps_m3b ;
+         label := label_vc_sys_seq
+     |}.
+ 
+     Definition steps_m4b : list (states_vc_sys_seq * states_vc_sys_seq) := 
+         (vc_sys_vc, vc_sys_ms3) ::
+         (vc_sys_c, vc_sys_ms3) ::
+         (vc_sys_ms3, vc_sys_ms4) :: 
+         (vc_sys_sys, vc_sys_ms4) ::
+         nil.
+ 
+     Definition m4b : attackgraph measurement adversary := 
+     {|
+         event := states_vc_sys_seq ;
+         edges := steps_m4b ;
+         label := label_vc_sys_seq
+     |}.
+ 
+     (* Prove m2b, m3b and m4b reduce *)
+ 
+     Definition steps_m2b' : list (states_vc_sys_seq * states_vc_sys_seq) := 
+         (vc_sys_vc, vc_sys_ms4) ::
+         (vc_sys_sys, vc_sys_ms4) ::
+         nil.
+ 
+     Definition m2b' : attackgraph measurement adversary := 
+     {|
+         event := states_vc_sys_seq ;
+         edges := steps_m2b' ;
+         label := label_vc_sys_seq
+     |}.
+ 
+     Definition steps_m3b' : list (states_vc_sys_seq * states_vc_sys_seq) := 
+         (vc_sys_vc, vc_sys_ms4) ::
+         (vc_sys_a, vc_sys_ms4) ::
+         (vc_sys_sys, vc_sys_ms4) ::
+         nil.
+ 
+     Definition m3b' : attackgraph measurement adversary := 
+     {|
+         event := states_vc_sys_seq ;
+         edges := steps_m3b' ;
+         label := label_vc_sys_seq
+     |}.
+ 
+     Definition steps_m4b' : list (states_vc_sys_seq * states_vc_sys_seq) := 
+         (vc_sys_vc, vc_sys_ms4) ::
+         (vc_sys_c, vc_sys_ms4) ::
+         (vc_sys_sys, vc_sys_ms4) ::
+         nil.
+ 
+     Definition m4b' : attackgraph measurement adversary := 
+     {|
+         event := states_vc_sys_seq ;
+         edges := steps_m4b' ;
+         label := label_vc_sys_seq
+     |}.
+ 
+     Lemma eqDec_measurement : forall (x y : measurement), {x = y} + {x <> y}.
+     Proof. destruct x, y; try (left; reflexivity); try (right; intros contra; inversion contra). Qed.
+     Lemma eqDec_adversary : forall (x y : adversary), {x = y} + {x <> y}.
+     Proof. destruct x, y; try (left; reflexivity); try (right; intros contra; inversion contra). Qed.
+     Lemma eqDec_event2: forall (x y : m2b.(event _ _)), {x = y} + {x <> y}.
+     Proof. destruct x, y; try (left; reflexivity); try (right; intros contra; inversion contra). Qed.
+     Lemma eqDec_event3: forall (x y : m3b.(event _ _)), {x = y} + {x <> y}.
+     Proof. destruct x, y; try (left; reflexivity); try (right; intros contra; inversion contra). Qed.
+     Lemma eqDec_event4: forall (x y : m4b.(event _ _)), {x = y} + {x <> y}.
+     Proof. destruct x, y; try (left; reflexivity); try (right; intros contra; inversion contra). Qed.
+ 
+     Ltac eqDec_edge_left step1 step2 eqDec_event :=
+     destruct (eqDec_edge eqDec_event step1 step2) as [H|H]; [clear H | contradiction].
+     Ltac eqDec_edge_right step1 step2 eqDec_event :=
+     destruct (eqDec_edge eqDec_event step1 step2) as [H|H]; [inversion H | clear H].
+     Ltac eqDec_event_left st1 st2 eqDec_event :=
+     destruct (eqDec_event st1 st2) as [H|H]; [clear H | contradiction].
+     Ltac eqDec_event_right st1 st2 eqDec_event :=
+     destruct (eqDec_event st1 st2) as [H|H]; [inversion H | clear H].
+ 
+     Lemma example_m2b_reduce1 : 
+     reduce1 eqDec_event2 steps_m2b =
+     steps_m2b'.
+     Proof.
+      unfold reduce1. simpl. 
+      eqDec_edge_left (vc_sys_ms3, vc_sys_ms4) (vc_sys_ms3, vc_sys_ms4) eqDec_event2.
+      eqDec_edge_right (vc_sys_ms3, vc_sys_ms4) (vc_sys_vc, vc_sys_ms4) eqDec_event2.
+      eqDec_edge_right (vc_sys_ms3, vc_sys_ms4) (vc_sys_sys, vc_sys_ms4) eqDec_event2.
       simpl.
-      eqDec_state_right c m.
-      eqDec_state_right m m'.
-      eqDec_state_right m' m.
-      eqDec_state_right v m.
-      eqDec_state_right m4 m.
-      eqDec_state_right s m.
-      intros contra. inversion contra.
-    + econstructor.
-    ++ unfold m5c_steps. simpl. unfold reduce1. simpl.
-        eqDec_step_right (m, m') (c, m').
-        eqDec_step_left (m, m') (m, m').
-        eqDec_step_right (m, m') (v, m').
-        eqDec_step_right (m, m') (m', m4).
-        eqDec_step_right (m, m') (s, m4).
-        unfold replace_measurement.
-        eqDec_state_right c m.
-        eqDec_state_right m' m.
-        eqDec_state_right v m.
-        eqDec_state_right m4 m.
-        eqDec_state_right s m.
-        simpl.
-        eqDec_step_right (m', m4) (c, m').
-        eqDec_step_right (m', m4) (v, m').
-        eqDec_step_left (m', m4) (m', m4).
-        eqDec_step_right (m', m4) (s, m4).
-        simpl.
-        eqDec_state_right c m'.
-        eqDec_state_left m' m'.
-        eqDec_state_right v m'.
-        eqDec_state_right s m'.
-        eqDec_state_right m4 m'.
-        intros contra. inversion contra.
-    ++ unfold m5c_steps. rewrite example_m5c'.
-       econstructor. unfold reduce1.
-       simpl. reflexivity.
-    Qed.
-
-End m5c.
+      eqDec_event_right vc_sys_vc vc_sys_ms3 eqDec_event2.
+      eqDec_event_right vc_sys_ms4 vc_sys_ms3 eqDec_event2.
+      eqDec_event_right vc_sys_sys vc_sys_ms3 eqDec_event2.
+      unfold steps_m2b'. reflexivity.
+     Qed. 
+ 
+     Lemma m2b_reduced : reducer eqDec_event2 steps_m2b steps_m2b'.
+     Proof. 
+         apply reduce_more.
+         + rewrite example_m2b_reduce1. unfold not. intros. inversion H. 
+         + rewrite example_m2b_reduce1. apply reduce_done. eauto.
+     Qed. 
+ 
+     Lemma example_m3b_reduce1 : 
+     reduce1 eqDec_event3 steps_m3b =
+     steps_m3b'.
+     Proof.
+      unfold reduce1. simpl. 
+      eqDec_edge_right (vc_sys_ms3, vc_sys_ms4) (vc_sys_vc, vc_sys_ms3) eqDec_event3.
+      eqDec_edge_right (vc_sys_ms3, vc_sys_ms4) (vc_sys_a, vc_sys_ms3) eqDec_event3.
+      eqDec_edge_left (vc_sys_ms3, vc_sys_ms4) (vc_sys_ms3, vc_sys_ms4) eqDec_event3.
+      eqDec_edge_right (vc_sys_ms3, vc_sys_ms4) (vc_sys_sys, vc_sys_ms4) eqDec_event3.
+      simpl.
+      eqDec_event_right vc_sys_vc vc_sys_ms3 eqDec_event3.
+      eqDec_event_right vc_sys_a vc_sys_ms3 eqDec_event3.
+      eqDec_event_left vc_sys_ms3 vc_sys_ms3 eqDec_event3.
+      eqDec_event_right vc_sys_sys vc_sys_ms3 eqDec_event3.
+      eqDec_event_right vc_sys_ms4 vc_sys_ms3 eqDec_event3.
+      unfold steps_m3b'. reflexivity.
+     Qed. 
+ 
+     Lemma m3b_reduced : reducer eqDec_event3 steps_m3b steps_m3b'.
+     Proof. 
+         apply reduce_more.
+         + rewrite example_m3b_reduce1. unfold not. intros. inversion H. 
+         + rewrite example_m3b_reduce1. apply reduce_done. eauto.
+     Qed. 
+ 
+     Lemma example_m4b_reduce1 : 
+     reduce1 eqDec_event4 steps_m4b =
+     steps_m4b'.
+     Proof.
+      unfold reduce1. simpl. 
+      eqDec_edge_right (vc_sys_ms3, vc_sys_ms4) (vc_sys_vc, vc_sys_ms3) eqDec_event4.
+      eqDec_edge_right (vc_sys_ms3, vc_sys_ms4) (vc_sys_c, vc_sys_ms3) eqDec_event4.
+      eqDec_edge_left (vc_sys_ms3, vc_sys_ms4) (vc_sys_ms3, vc_sys_ms4) eqDec_event4.
+      eqDec_edge_right (vc_sys_ms3, vc_sys_ms4) (vc_sys_sys, vc_sys_ms4) eqDec_event4.
+      simpl.
+      eqDec_event_right vc_sys_vc vc_sys_ms3 eqDec_event4.
+      eqDec_event_right vc_sys_c vc_sys_ms3 eqDec_event4.
+      eqDec_event_left vc_sys_ms3 vc_sys_ms3 eqDec_event4.
+      eqDec_event_right vc_sys_sys vc_sys_ms3 eqDec_event4.
+      eqDec_event_right vc_sys_ms4 vc_sys_ms3 eqDec_event4.
+      unfold steps_m4b'. reflexivity.
+     Qed. 
+ 
+     Lemma m4b_reduced : reducer eqDec_event4 steps_m4b steps_m4b'.
+     Proof. 
+         apply reduce_more.
+         + rewrite example_m4b_reduce1. unfold not. intros. inversion H. 
+         + rewrite example_m4b_reduce1. apply reduce_done. eauto.
+     Qed.
+ 
+     (* define isomorphism function *)
+     Definition f (x : states_sys) : states_vc_sys_seq :=
+         match x with 
+         | sys_sys => vc_sys_sys 
+         | sys_vc => vc_sys_vc
+         | sys_ker => vc_sys_ker
+         | sys_a => vc_sys_a
+         | sys_c => vc_sys_c
+         | sys_ms3 => vc_sys_ms3
+         | sys_ms4 => vc_sys_ms4
+     end.
+ 
+     Definition g (x : states_vc_sys_seq) : option (states_sys) :=
+         match x with 
+         | vc_sys_sys => Some sys_sys 
+         | vc_sys_vc => Some sys_vc
+         | vc_sys_ker => Some sys_ker
+         | vc_sys_ms4 => Some sys_ms4
+         | _ => None
+     end.
+ 
+     Definition g' (x : states_vc_sys_seq) : (states_sys) :=
+         match x with 
+         | vc_sys_sys =>  sys_sys 
+         | vc_sys_vc =>  sys_vc
+         | vc_sys_ker =>  sys_ker
+         | vc_sys_ms4 =>  sys_ms4
+         | _ => sys_ms4
+     end.
+     
+     Definition sys_all : list (attackgraph measurement adversary) :=  m1a :: m2a :: nil .
+ 
+     Definition vc_sys_seq_all := m1b :: m2b' :: m3b' :: m4b' :: nil.
+ 
+     Ltac cor_in_head := simpl; apply ex_head; auto.
+     Ltac cor_in_tail := simpl; apply ex_tail; auto.
+ 
+     Lemma m1a_supports_m1b : supports ( m1a :: nil ) (m1b :: nil).
+     Proof.
+         unfold supports. intros. simpl in H0. intuition. 
+         exists m1a. simpl in *. split.
+         + left. reflexivity.
+         + right. subst. unfold strict_partial_order. intuition.
+         ++ econstructor.
+         +++ simpl. unfold steps_m1b. apply ex_tail. apply ex_tail. apply ex_head. simpl. intuition.
+         +++  econstructor. simpl. unfold steps_m1b. apply ex_tail. apply ex_head. simpl. eauto. econstructor.
+         ++ econstructor.
+         +++ simpl. unfold steps_m1b. unfold find_time. simpl. eauto.
+         +++ econstructor. simpl. unfold steps_m1b. unfold find_time. simpl. eauto.
+             econstructor.
+         ++ right. unfold time_proper_subset. split.
+         +++ econstructor.
+         ++++ simpl. unfold steps_m1b. unfold find_time. simpl. eauto.
+         ++++ econstructor. simpl. unfold steps_m1b. unfold find_time. simpl. eauto.
+             econstructor.
+         +++ unfold not. intros. invc H. subst. simpl in *. invc H2. subst.
+             simpl in *. destruct H0. inversion H0. subst. invc H0. subst. 
+             destruct H1. simpl in *. invc H. subst. invc H1.
+     Qed.
+ 
+     Ltac inversion_any :=
+       match goal with
+       | [H : _ |- _ ] => inversion H
+       end.
+ 
+     Lemma vc_sys_seq_supports_sys : supports sys_all vc_sys_seq_all.
+     Proof.
+       unfold supports. intros. simpl in H0. intuition.
+       + subst. exists m1a. unfold sys_all; intuition. right.
+         unfold strict_partial_order. intuition.
+       ++ econstructor. 
+       +++ simpl. unfold steps_m1b. apply ex_tail. apply ex_tail. apply ex_head. simpl. intuition.
+       +++ econstructor. simpl. unfold steps_m1b. apply ex_tail. apply ex_head. simpl. eauto. econstructor.
+       ++ econstructor.
+       +++ simpl. unfold steps_m1b. unfold find_time. simpl. eauto.
+       +++ econstructor. simpl. unfold steps_m1b. unfold find_time. simpl. eauto.
+           econstructor.
+       ++ right. unfold time_proper_subset. split.
+       +++ econstructor.
+       ++++ simpl. unfold steps_m1b. unfold find_time. simpl. eauto.
+       ++++ econstructor. simpl. unfold steps_m1b. unfold find_time. simpl. eauto.
+           econstructor.
+       +++ unfold not. intros. invc H. subst. simpl in *. invc H2. subst.
+           simpl in *. destruct H0. inversion H0. subst. invc H0. subst. 
+           destruct H1. simpl in *. invc H. subst. invc H1.
+       + subst. exists m1a. unfold sys_all. intuition. left.
+         unfold isomorphism. exists f. unfold f. repeat split; intros.
+       ++ destruct st1, st2; try (simpl in *; intuition; inversion_any).
+       ++ destruct st1, st2; try (simpl in *; intuition; inversion_any).
+       ++ destruct st; auto.
+       ++ destruct st1, st2; try reflexivity; inversion_any.
+       ++ destruct st'.
+       +++ exists sys_sys; reflexivity.
+       +++ exists sys_ker; reflexivity.
+       +++ exists sys_vc; reflexivity.
+       +++ exists sys_a; reflexivity.
+       +++ exists sys_c; reflexivity.
+       +++ exists sys_ms3; reflexivity.
+       +++ exists sys_ms4; reflexivity.
+       + exists m1a. unfold sys_all. intuition. right. subst.
+         unfold strict_partial_order. intuition. 
+       ++  econstructor. 
+       +++ simpl. unfold steps_m3b'. apply ex_tail. apply ex_tail. apply ex_head. simpl. intuition.
+       +++ econstructor. simpl. unfold steps_m3b'. apply ex_head. simpl. eauto. econstructor.
+       ++ econstructor.
+       +++ simpl. unfold steps_m3b'. unfold find_time. simpl. eauto.
+       +++ econstructor. simpl. unfold steps_m3b'. unfold find_time. simpl. eauto.
+           econstructor.
+       ++ left. unfold cor_proper_subset. intuition.
+       +++ econstructor.  
+       ++++ simpl. unfold steps_m3b'. apply ex_tail. apply ex_tail. apply ex_head. simpl. intuition.
+       ++++ econstructor. simpl. unfold steps_m3b'. apply ex_head. simpl. eauto. econstructor.
+       +++ invc H. subst. invc H4. subst. invc H1. subst. invc H0.
+           subst. invc H0. subst. invc H1. invc H1.
+       +  exists m1a. unfold sys_all. intuition. right. subst.
+       unfold strict_partial_order. intuition. 
+     ++  econstructor. 
+     +++ simpl. unfold steps_m3b'. apply ex_tail. apply ex_tail. apply ex_head. simpl. intuition.
+     +++ econstructor. simpl. unfold steps_m3b'. apply ex_head. simpl. eauto. econstructor.
+     ++ econstructor.
+     +++ simpl. unfold steps_m3b'. unfold find_time. simpl. eauto.
+     +++ econstructor. simpl. unfold steps_m3b'. unfold find_time. simpl. eauto.
+         econstructor.
+     ++ left. unfold cor_proper_subset. intuition.
+     +++ econstructor.  
+     ++++ simpl. unfold steps_m3b'. apply ex_tail. apply ex_tail. apply ex_head. simpl. intuition.
+     ++++ econstructor. simpl. unfold steps_m3b'. apply ex_head. simpl. eauto. econstructor.
+     +++ invc H. subst. invc H4. subst. invc H1. subst. invc H0.
+         subst. invc H0. subst. invc H1. invc H1.
+  Qed.
+ 
+  (* TO DO... random example. Not part of dissertation. *)
+  (*
+  Theorem vc_sys_seq_set_reduced : reduce_set vc_sys_seq_all vc_sys_seq_all (m2b' :: nil).
+  Proof.
+     unfold vc_sys_seq_all. apply set_remove. 
+     + exists m2b'. split; auto with *.  admit.
+     + apply set_keep.
+     ++ intros. simp_int.
+     +++ subst. unfold strict_partial_order in H0. invc H0. admit.
+     +++ subst.  admit.
+     +++ admit. 
+     +++ admit.
+     ++  apply set_remove. 
+     +++ exists m2b'.  admit.
+     +++ apply set_remove. 
+     ++++ admit.
+     ++++ apply set_nil.     
+ Admitted.
+*)
+ 
+ End vc_sys_seq_supports_sys. 
+ 
+ 
+ (* *********** *)
+ (* Example m2c *)
+ (* *********** *)
+ (* *********** *)
+ 
+ Module m3b.
+ 
+     Set Implicit Arguments.
+     
+     Inductive measurement : Type :=
+     | ms : measurement
+     | ms4 : measurement.
+     
+     Inductive adversary : Type :=
+     | sys : adversary
+     | ker : adversary.
+     
+     Inductive state_m3b : Type :=
+     | s : state_m3b 
+     | k : state_m3b
+     | m : state_m3b
+     | m4 : state_m3b.
+     
+     Definition label_m3b (st : state_m3b) : measurement + adversary :=
+     match st with
+     | s => inr sys
+     | k => inr ker
+     | m => inl ms
+     | m4 => inl ms4
+     end.
+     
+     Definition steps_m3b : list (state_m3b * state_m3b) := 
+         (k, m) :: 
+         (m, m4) ::
+         (s, m4) ::
+         nil.
+     
+     Definition m3b : attackgraph measurement adversary := 
+     {|
+         event := state_m3b ;
+         edges := steps_m3b ;
+         label := label_m3b
+     |}.
+     
+     Lemma eqDec_measurement : forall (x y : measurement), {x = y} + {x <> y}.
+     Proof. destruct x, y; try (left; reflexivity); try (right; intros contra; inversion contra). Qed.
+     Lemma eqDec_adversary : forall (x y : adversary), {x = y} + {x <> y}.
+     Proof. destruct x, y; try (left; reflexivity); try (right; intros contra; inversion contra). Qed.
+     Lemma eqDec_event: forall (x y : m3b.(event _ _)), {x = y} + {x <> y}.
+     Proof. destruct x, y; try (left; reflexivity); try (right; intros contra; inversion contra). Qed.
+ 
+     Ltac eqDec_edge_left step1 step2 :=
+     destruct (eqDec_edge eqDec_event step1 step2) as [H|H]; [clear H | contradiction].
+     Ltac eqDec_edge_right step1 step2 :=
+     destruct (eqDec_edge eqDec_event step1 step2) as [H|H]; [inversion H | clear H].
+     Ltac eqDec_event_left st1 st2 :=
+     destruct (eqDec_event st1 st2) as [H|H]; [clear H | contradiction].
+     Ltac eqDec_event_right st1 st2 :=
+     destruct (eqDec_event st1 st2) as [H|H]; [inversion H | clear H].
+ 
+     Print reduce1.
+ 
+     Lemma example_m3b : 
+     (reduce1 eqDec_event m3b.(edges _ _)) =
+     ((k, m4) :: (s, m4) :: nil).
+     Proof.
+         unfold reduce1.
+         simpl. 
+         eqDec_edge_right (m, m4) (k, m).
+         eqDec_edge_left (m, m4) (m, m4).
+         eqDec_edge_right (m, m4) (s, m4).
+         simpl.
+         eqDec_event_right k m.
+         eqDec_event_left m m.
+         eqDec_event_right s m.
+         eqDec_event_right m4 m.
+         eauto.
+     Qed.
+ 
+     Definition m3b_edges := m3b.(edges _ _).
+     Definition m3b_reduced := ((k, m4) :: (s, m4) :: nil).
+ 
+     Check reducer eqDec_event m3b_edges m3b_reduced. 
+ 
+     Lemma example_m3b_reducer : 
+         reducer eqDec_event m3b_edges m3b_reduced.
+     Proof.
+         econstructor.
+         + unfold m3b_edges. rewrite example_m3b. simpl. intros contra. inversion contra.
+         + unfold m3b_edges. rewrite example_m3b.
+           apply reduce_done. unfold reduce1. simpl. eauto.
+     Qed.
+     
+ 
+ End m3b.
+ 
+ 
+ (* *********** *)
+ (* Example m2c *)
+ (* *********** *)
+ (* *********** *)
+ Module m2c.
+ 
+ Inductive measurement : Type :=
+ | ms : measurement
+ | ms4 : measurement.
+ 
+ Inductive adversary : Type :=
+ | sys : adversary
+ | ker : adversary.
+ 
+ Inductive state_m2c : Type :=
+ | s : state_m2c
+ | k : state_m2c
+ | m : state_m2c
+ | m' : state_m2c
+ | m4 : state_m2c.
+ 
+ Definition label_m2c (st : state_m2c) : measurement + adversary :=
+ match st with
+ | s => inr sys
+ | k => inr ker
+ | m => inl ms
+ | m' => inl ms
+ | m4 => inl ms4
+ end.
+ 
+ Definition steps_m2c : list (state_m2c * state_m2c) :=  
+     (m, m') ::
+     (m', k) ::
+     (s, m4) :: 
+     (k, m4) :: 
+     nil.
+ 
+ Definition steps_m2b : list (state_m2c * state_m2c) :=  
+     (m', k) ::
+     (s, m4) :: 
+     (k, m4) :: 
+     nil.
+ 
+ Definition steps_m2a : list (state_m2c * state_m2c) :=  
+     (s, m4) :: 
+     (k, m4) :: 
+     nil.
+ 
+ 
+ Definition m2c : attackgraph measurement adversary := 
+ {|
+     event := state_m2c ;
+     edges := steps_m2c ;
+     label := label_m2c
+ |}.
+ 
+ Definition m2b : attackgraph measurement adversary := 
+ {|
+     event := state_m2c ;
+     edges := steps_m2b ;
+     label := label_m2c
+ |}.
+ 
+ Definition m2a : attackgraph measurement adversary := 
+ {|
+     event := state_m2c ;
+     edges := steps_m2a ;
+     label := label_m2c
+ |}.
+ 
+ Definition m2a_nil : attackgraph measurement adversary := 
+ {|
+     event := state_m2c ;
+     edges := nil ;
+     label := label_m2c
+ |}.
+ 
+ 
+ Lemma eqDec_measurement : forall (x y : measurement), {x = y} + {x <> y}.
+ Proof. destruct x, y; try (left; reflexivity); try (right; intros contra; inversion contra). Qed.
+ Lemma eqDec_adversary : forall (x y : adversary), {x = y} + {x <> y}.
+ Proof. destruct x, y; try (left; reflexivity); try (right; intros contra; inversion contra). Qed.
+ Lemma eqDec_event : forall (x y : m2c.(event _ _)), {x = y} + {x <> y}.
+ Proof. destruct x, y; try (left; reflexivity); try (right; intros contra; inversion contra). Qed.
+ 
+ Ltac eqDec_edge_left step1 step2 :=
+     destruct (eqDec_edge eqDec_event step1 step2) as [H|H]; [clear H | contradiction].
+ Ltac eqDec_edge_right step1 step2 :=
+     destruct (eqDec_edge eqDec_event step1 step2) as [H|H]; [inversion H | clear H].
+ Ltac eqDec_event_left st1 st2 :=
+     destruct (eqDec_event st1 st2) as [H|H]; [clear H | contradiction].
+ Ltac eqDec_event_right st1 st2 :=
+     destruct (eqDec_event st1 st2) as [H|H]; [inversion H | clear H].
+ 
+ Lemma example_m2c : 
+     (reduce1 eqDec_event m2c.(edges _ _)) =
+     ((m', k) :: (s, m4) :: (k, m4) :: nil).
+ Proof.
+     unfold reduce1.
+     simpl. 
+     eqDec_edge_left (m, m') (m, m').
+     eqDec_edge_right (m, m') (m', k).
+     eqDec_edge_right (m, m') (s, m4).
+     eqDec_edge_right (m, m') (k, m4).
+     simpl.
+     eqDec_event_right m' m.
+     eqDec_event_right k m.
+     eqDec_event_right s m.
+     eqDec_event_right m4 m.
+     reflexivity.
+ Qed.
+ 
+ Print time_subset. 
+ Lemma time_subset_m2a_m2c : time_subset m2a.(edges _ _) m2c.(edges _ _).
+ Proof.
+     simpl. auto.
+ Qed.
+ 
+ (* TODO: this proof?? *)
+ Lemma not_time_subset_m2c_m2a : ~ time_subset m2c.(edges _ _) m2a.(edges _ _).
+ Proof.
+     unfold not; intros.
+     inversion H. inversion H0.
+     inversion H2. clear H2.
+ Abort.
+ 
+ (* TODO: this proof too? *)
+ Lemma subset_nil : ~ cor_subset m2a.(edges _ _) m2a_nil.(edges _ _).
+ Proof.
+ Abort.
+ 
+ (* TODO *)
+ Lemma subset_nil_with_meas : ~ cor_subset m2c.(edges _ _) m2a_nil.(edges _ _).
+ Proof.
+ Abort.
+ 
+ End m2c.
+ 
+ (* *********** *)
+ (* Example m5c *)
+ (* *********** *)
+ (* *********** *)
+ Module m5c.
+ 
+ Inductive measurement : Type :=
+ | ms : measurement
+ | ms4 : measurement.
+ 
+ Inductive adversary : Type :=
+ | sys : adversary
+ | vc : adversary
+ | cc : adversary.
+ 
+ Inductive state_m5c : Type :=
+ | s : state_m5c
+ | v : state_m5c
+ | c : state_m5c
+ | m : state_m5c
+ | m' : state_m5c
+ | m4 : state_m5c.
+ 
+ Definition label_m5c (st : state_m5c) : measurement + adversary :=
+ match st with
+ | s => inr sys
+ | v => inr vc
+ | c => inr cc
+ | m => inl ms
+ | m' => inl ms
+ | m4 => inl ms4
+ end.
+ 
+ Definition steps_m5c : list (state_m5c * state_m5c) := 
+     (c, m') ::
+     (m, m') ::
+     (v, m') ::
+     (m', m4) ::
+     (s, m4) ::
+     nil.
+ 
+ Definition m5c : attackgraph measurement adversary := 
+ {|
+     event := state_m5c ;
+     edges := steps_m5c ;
+     label := label_m5c
+ |}.
+ 
+ (* remove c to m' to have a proper subset *)
+ Definition steps_m5c' : list (state_m5c * state_m5c) := 
+     (m, m') ::
+     (v, m') ::
+     (m', m4) ::
+     (s, m4) ::
+     nil.
+ 
+ (* new graph that would be proper subset *)
+ Definition m5c' : attackgraph measurement adversary := 
+ {|
+     event := state_m5c ;
+     edges := steps_m5c' ;
+     label := label_m5c
+ |}.
+ 
+ Lemma eqDec_measurement : forall (x y : measurement), {x = y} + {x <> y}.
+ Proof. destruct x, y; try (left; reflexivity); try (right; intros contra; inversion contra). Qed.
+ Lemma eqDec_adversary : forall (x y : adversary), {x = y} + {x <> y}.
+ Proof. destruct x, y; try (left; reflexivity); try (right; intros contra; inversion contra). Qed.
+ Lemma eqDec_event : forall (x y : m5c.(event _ _)), {x = y} + {x <> y}.
+ Proof. destruct x, y; try (left; reflexivity); try (right; intros contra; inversion contra). Qed.
+ 
+ 
+ Ltac eqDec_edge_left step1 step2 :=
+     destruct (eqDec_edge eqDec_event step1 step2) as [H|H]; [clear H | contradiction].
+ Ltac eqDec_edge_right step1 step2 :=
+     destruct (eqDec_edge eqDec_event step1 step2) as [H|H]; [inversion H | clear H].
+ Ltac eqDec_event_left st1 st2 :=
+     destruct (eqDec_event st1 st2) as [H|H]; [clear H | contradiction].
+ Ltac eqDec_event_right st1 st2 :=
+     destruct (eqDec_event st1 st2) as [H|H]; [inversion H | clear H].
+     
+ Definition m5c_edges := m5c.(edges _ _).
+ Definition m5c'_edges := m5c'.(edges _ _).
+ Definition m5c_reduced := ((c, m4) :: (v, m4) :: (s, m4) :: nil).
+ 
+ (* must call reduce1 twice here *)
+ Lemma example_m5c' : 
+     (reduce1 eqDec_event (reduce1 eqDec_event m5c.(edges _ _))) =
+     ((c, m4) :: (v, m4) :: (s, m4) :: nil).
+ Proof.
+     unfold reduce1.
+     simpl.
+     eqDec_edge_right (m, m') (c, m').
+     eqDec_edge_left (m, m') (m, m').
+     eqDec_edge_right (m, m') (v, m').
+     eqDec_edge_right (m, m') (m', m4).
+     eqDec_edge_right (m, m') (s, m4).
+     simpl.
+     eqDec_event_right c m.
+     eqDec_event_right v m.
+     eqDec_event_right m' m.
+     eqDec_event_right m4 m.
+     eqDec_event_right s m.
+     simpl.
+     eqDec_edge_right (m', m4) (c, m').
+     eqDec_edge_right (m', m4) (v, m').
+     eqDec_edge_left (m', m4) (m', m4).
+     eqDec_edge_right (m', m4) (s, m4).
+     simpl.
+     eqDec_event_right c m'.
+     eqDec_event_left m' m'.
+     eqDec_event_right v m'.
+     eqDec_event_right s m'.
+     eqDec_event_right m4 m'.
+     reflexivity.
+ Qed.
+ 
+ Lemma example_m5c_reducer : 
+ reducer eqDec_event m5c_edges m5c_reduced.
+ Proof.
+     econstructor.
+     + unfold m5c_edges. simpl. unfold reduce1. simpl. 
+       eqDec_edge_right (m, m') (c, m').
+       eqDec_edge_left (m, m') (m, m').
+       eqDec_edge_right (m, m') (v, m').
+       eqDec_edge_right (m, m') (m', m4).
+       eqDec_edge_right (m, m') (s, m4).
+       simpl.
+       eqDec_event_right c m.
+       eqDec_event_right m m'.
+       eqDec_event_right m' m.
+       eqDec_event_right v m.
+       eqDec_event_right m4 m.
+       eqDec_event_right s m.
+       intros contra. inversion contra.
+     + econstructor.
+     ++ unfold m5c_edges. simpl. unfold reduce1. simpl.
+         eqDec_edge_right (m, m') (c, m').
+         eqDec_edge_left (m, m') (m, m').
+         eqDec_edge_right (m, m') (v, m').
+         eqDec_edge_right (m, m') (m', m4).
+         eqDec_edge_right (m, m') (s, m4).
+         unfold replace_measurement.
+         eqDec_event_right c m.
+         eqDec_event_right m' m.
+         eqDec_event_right v m.
+         eqDec_event_right m4 m.
+         eqDec_event_right s m.
+         simpl.
+         eqDec_edge_right (m', m4) (c, m').
+         eqDec_edge_right (m', m4) (v, m').
+         eqDec_edge_left (m', m4) (m', m4).
+         eqDec_edge_right (m', m4) (s, m4).
+         simpl.
+         eqDec_event_right c m'.
+         eqDec_event_left m' m'.
+         eqDec_event_right v m'.
+         eqDec_event_right s m'.
+         eqDec_event_right m4 m'.
+         intros contra. inversion contra.
+     ++ unfold m5c_edges. rewrite example_m5c'.
+        econstructor. unfold reduce1.
+        simpl. reflexivity.
+     Qed.
+ 
+ End m5c.
