src/coq_formalism/graph_normalization.v
@@ -22,96 +22,96 @@ Section Reducer.
     (* Labels and States must have decidable equality *)
     Hypothesis eqDec_measurement : forall (x y : measurement), {x = y} + {x <> y}.
     Hypothesis eqDec_adversary : forall (x y : adversary), {x = y} + {x <> y}.
-    Hypothesis eqDec_state :  forall (x y : G.(state _ _)), {x = y} + {x <> y}.
+    Hypothesis eqDec_event :  forall (x y : G.(event _ _)), {x = y} + {x <> y}.
 
-    (* steps are equivalent or not equivalent *)
-    Lemma eqDec_step : forall (x y : (G.(state _ _) * G.(state _ _))), {x = y} + {x <> y}.
+    (* edges are equivalent or not equivalent *)
+    Lemma eqDec_edge : forall (x y : (G.(event _ _) * G.(event _ _))), {x = y} + {x <> y}.
     Proof.
         intros x y;
         destruct x as [stx stx']; destruct y as [sty sty'].
-        destruct eqDec_state with (x:=stx) (y:=sty).
-        + destruct eqDec_state with (x:=stx') (y:=sty').
+        destruct eqDec_event with (x:=stx) (y:=sty).
+        + destruct eqDec_event with (x:=stx') (y:=sty').
         ++ subst. left. eauto.  
         ++ right. intros contra. rewrite pair_equal_spec in contra. destruct contra. contradiction.
-        + destruct eqDec_state with (x:=stx') (y:=sty').
+        + destruct eqDec_event with (x:=stx') (y:=sty').
         ++ right. intros contra. rewrite pair_equal_spec in contra. destruct contra. contradiction.
         ++ right. intros contra. rewrite pair_equal_spec in contra. destruct contra. contradiction.
     Qed.
 
-    (* list of steps are decidably equal *)
-    Lemma eqDec_list_steps: forall (x y : list (G.(state _ _) * G.(state _ _))), {x = y} + {x <> y}.
+    (* list of edges are decidably equal *)
+    Lemma eqDec_list_edges : forall (x y : list (G.(event _ _) * G.(event _ _))), {x = y} + {x <> y}.
     Proof.
-        intros G0. apply list_eq_dec. apply eqDec_step.
+        intros G0. apply list_eq_dec. apply eqDec_edge.
     Qed.
 
-    Fixpoint replace_measurement_incomplete (Steps : list (G.(state _ _) * G.(state _ _))) (st st' : (G.(state _ _))) : 
-                                 list (G.(state _ _) * G.(state _ _)) := 
-        match Steps with 
-        | (st1, st2) :: Steps' => if (eqDec_state st st2)
-                                  then (st1, st') :: replace_measurement_incomplete Steps' st st' 
-                                  else (st1, st2) :: replace_measurement_incomplete Steps' st st'
-        | nil => Steps 
+    Fixpoint replace_measurement_incomplete (edges : list (G.(event _ _) * G.(event _ _))) (st st' : (G.(event _ _))) : 
+                                 list (G.(event _ _) * G.(event _ _)) := 
+        match edges with 
+        | (st1, st2) :: edges' => if (eqDec_event st st2)
+                                  then (st1, st') :: replace_measurement_incomplete edges' st st' 
+                                  else (st1, st2) :: replace_measurement_incomplete edges' st st'
+        | nil => edges 
         end. 
 
-    (* Replace all occurences of st by st' in Steps *)
-    Fixpoint replace_measurement (Steps : list (G.(state _ _) * G.(state _ _))) 
-    (st st' : G.(state _ _)) : 
-    list (G.(state _ _) * G.(state _ _)) :=
-    match Steps with
-    | (st1, st2) :: Steps' => 
-        if (eqDec_state st1 st)
-        then if (eqDec_state st2 st)
-            then (st', st') :: replace_measurement Steps' st st'
-            else (st', st2) :: replace_measurement Steps' st st'
-        else if (eqDec_state st2 st)
-            then (st1, st') :: replace_measurement Steps' st st'
-            else (st1, st2) :: replace_measurement Steps' st st'
-    | nil => Steps
+    (* Replace all occurences of st by st' in edges *)
+    Fixpoint replace_measurement (edges : list (G.(event _ _) * G.(event _ _))) 
+    (st st' : G.(event _ _)) : 
+    list (G.(event _ _) * G.(event _ _)) :=
+    match edges with
+    | (st1, st2) :: edges' => 
+        if (eqDec_event st1 st)
+        then if (eqDec_event st2 st)
+            then (st', st') :: replace_measurement edges' st st'
+            else (st', st2) :: replace_measurement edges' st st'
+        else if (eqDec_event st2 st)
+            then (st1, st') :: replace_measurement edges' st st'
+            else (st1, st2) :: replace_measurement edges' st st'
+    | nil => edges
     end.
 
-    Fixpoint find_measurement (AllSteps Steps : list (G.(state _ _) * G.(state _ _))) :  list (G.(state _ _) * G.(state _ _)) := 
-    match Steps with 
-    | (st, st') :: Steps' => match (G.(label _ _) st) with 
-                             | inr c1 => find_measurement AllSteps Steps' 
+    Fixpoint find_measurement (Alledges edges : list (G.(event _ _) * G.(event _ _))) :  list (G.(event _ _) * G.(event _ _)) := 
+    match edges with 
+    | (st, st') :: edges' => match (G.(label _ _) st) with 
+                             | inr c1 => find_measurement Alledges edges' 
                              | inl m1 => match (G.(label _ _) st') with 
                                          (* if both m1 and m2 are measurement events then you can replace them *)
-                                         | inl m2 => replace_measurement (remove (eqDec_step ) (st, st') AllSteps) st st' 
-                                         | _ => find_measurement AllSteps Steps'
+                                         | inl m2 => replace_measurement (remove (eqDec_edge ) (st, st') Alledges) st st' 
+                                         | _ => find_measurement Alledges edges'
                                          end
                              end
-    | nil => AllSteps
+    | nil => Alledges
     end.
 
     (* finding measurement x in x should return x? *)
-    Lemma find_measurement_helper : forall (x : list(G.(state _ _) * G.(state _ _))), find_measurement x x = x.
+    Lemma find_measurement_helper : forall (x : list(G.(event _ _) * G.(event _ _))), find_measurement x x = x.
     Proof.
         intros. induction x.
         + auto.
         + (* simpl. destruct a. destruct (G.(label _ _) s) eqn:l_a .
         ++ destruct (G.(label _ _) s0) eqn:l_a2.
-        +++ simpl in *. destruct ((eqDec_step G) (s, s0) (s, s0)).
+        +++ simpl in *. destruct ((eqDec_edge G) (s, s0) (s, s0)).
         ++++ simpl. unfold remove. unfold replace_measurement.*)
     Abort.
 
-    Definition reduce1 (Steps : list (G.(state _ _) * G.(state _ _))) : list (G.(state _ _) * G.(state _ _)) :=
-    find_measurement Steps Steps.
+    Definition reduce1 (edges : list (G.(event _ _) * G.(event _ _))) : list (G.(event _ _) * G.(event _ _)) :=
+    find_measurement edges edges.
 
     (* We cannot define a recursive fixpoint because of 
      * Coq's termination checker since it's not obvious 
      * the list is getting smaller. Instead, we must write 
      * an inductively defined proposition to express that 
      * the graphs eventually reduce. This definition relies
-     * on reduce1 to state that if reduce1 returns itself 
+     * on reduce1 to event that if reduce1 returns itself 
      * then the graph cannot be further reduced. If reduce1
      * does not return itself, then the reduction call is
      * recursed. *)
-    Inductive reducer : list (G.(state _ _) * G.(state _ _)) -> list (G.(state _ _) * G.(state _ _)) -> Prop :=
+    Inductive reducer : list (G.(event _ _) * G.(event _ _)) -> list (G.(event _ _) * G.(event _ _)) -> Prop :=
     | reduce_done : forall x, reduce1 x = x -> reducer x x
     | reduce_more : forall x y, reduce1 x <> x -> reducer (reduce1 x) y -> reducer x y.  
 
-    Definition step_update (g1 : attackgraph measurement adversary) (newSteps : list (g1.(state _ _) * g1.(state _ _))) :=  {| state := g1.(state _ _) ; steps := newSteps ; label := g1.(label _ _) |}. 
+    Definition step_update (g1 : attackgraph measurement adversary) (newedges : list (g1.(event _ _) * g1.(event _ _))) :=  {| event := g1.(event _ _) ; edges := newedges ; label := g1.(label _ _) |}. 
 
-    Theorem  reducer_deterministic : forall (x y z : list (G.(state _ _) * G.(state _ _))), 
+    Theorem  reducer_deterministic : forall (x y z : list (G.(event _ _) * G.(event _ _))), 
         reducer x y -> reducer x z -> y = z.
     Proof.
         intros.
@@ -125,7 +125,7 @@ Section Reducer.
     Qed.
     
     (* if a graph reduces from x to y and then y to z then you can say x reduces to z *)
-    Theorem  reducer_trans : forall (x : list(G.(state _ _) * G.(state _ _))) (y : list(G.(state _ _) * G.(state _ _))) , reducer x y -> forall (z : list(G.(state _ _) * G.(state _ _))) , reducer y z -> reducer x z.
+    Theorem  reducer_trans : forall (x : list(G.(event _ _) * G.(event _ _))) (y : list(G.(event _ _) * G.(event _ _))) , reducer x y -> forall (z : list(G.(event _ _) * G.(event _ _))) , reducer y z -> reducer x z.
     Proof.
         intros x y Hxy. induction Hxy.
         + eauto.
